ironfleet/src/Dafny/Distributed/Impl/SHT/SingleDeliveryModel.i.dfy
@@ -229,7 +229,7 @@ method ReceiveSingleMessageImpl(acct:CSingleDeliveryAcct, pkt:CPacket, ghost par
 }
 
 
-method SendSingleCMessage(acct:CSingleDeliveryAcct, m:CMessage, dst:EndPoint, params:CParameters) 
+method {:timeLimitMultiplier 3} SendSingleCMessage(acct:CSingleDeliveryAcct, m:CMessage, dst:EndPoint, params:CParameters) 
     returns (acct':CSingleDeliveryAcct, sm:CSingleMessage, shouldSend:bool)
     requires CSingleDeliveryAccountIsValid(acct, params);
     requires CMessageIsAbstractable(m);
